ott_coq/destination_calculus_sugar_typing.v
@@ -1,0 +1,72 @@
+Require Import List.
+Require Import Ott.ott_list_core.
+Require Import Dest.destination_calculus_ott.
+Require Import Dest.destination_calculus_notations.
+Require Import Dest.ext_nat.
+Require Import Coq.Program.Equality.
+Require Import Dest.Finitely.
+From Hammer Require Import Hammer.
+From Hammer Require Import Tactics.
+(* ⬇️ for the `impl` relation. *)
+Require Coq.Program.Basics.
+Require Import Coq.Logic.Eqdep_dec.
+Require Import Coq.Logic.EqdepFacts.
+Require Import Coq.Logic.FunctionalExtensionality.
+Require Import Coq.Logic.ProofIrrelevance.
+Require Import Coq.Arith.Plus.
+Require Import Arith.
+Require Import Dest.destination_calculus_proofs.
+
+Theorem Ty_termS_Alloc : forall (P : ctx) (T : type), DisposableOnly P -> P ⊢ alloc : T ⧔ (⌊ T ⌋ ¹ν).
+Proof.
+  intros P T DisposP.
+  unfold termS_Alloc.
+  rewrite union_empty_r_eq with (G := P).
+  apply Ty_term_Val.
+  - assumption.
+  - rewrite union_empty_r_eq with (G := ᴳ{}).
+    assert (hvarsᴳ(ᴳ- ᴳ{+ 1 : ¹ν ⌊ T ⌋ ¹ν }) = ᴴ{ 1}) as hvarsD3Eq.
+      { rewrite hvars_minus_eq. unfold hvars_ctx, hvars_dom, ctx_singleton, hminus. rewrite dom_singleton_eq. cbn. reflexivity. }
+    rewrite <- hvarsD3Eq. apply TyR_val_A; swap 1 10; swap 2 11.
+    + rewrite stimes_empty_eq, <- union_empty_l_eq. apply TyR_val_D.
+    + rewrite <- union_empty_l_eq. rewrite hminus_singleton. apply TyR_val_H.
+    + apply DestOnly_singleton_dest.
+    + apply LinOnly_singleton_iff. cbn. constructor.
+    + apply FinAgeOnly_singleton_iff. cbn. constructor.
+    + apply ValidOnly_singleton_iff. cbn. constructor.
+    + apply Disjoint_empty_l.
+    + apply Disjoint_empty_l.
+    + apply Disjoint_empty_l.
+    + apply DestOnly_empty.
+    + apply DestOnly_empty.
+  - + apply DestOnly_empty.
+Qed.
+
+Theorem Ty_termS_FromA' : forall (P : ctx) (t : term) (T : type), P ⊢ t : T ⧔ ① -> P ⊢ from⧔' t : T.
+Proof.
+  intros * Tyt.
+  unfold termS_FromA'.
+  replace P with (¹ν ᴳ· P ᴳ+ ᴳ{}). 2:{ crush. }
+  apply Ty_term_PatP with (T1 := T) (T2 := ! ¹∞ ⁔ ①).
+  - constructor.
+  - apply Disjoint_empty_l.
+  - apply Disjoint_empty_l.
+  - apply Disjoint_singletons_iff. sfirstorder.
+  - apply Ty_term_FromA.
+    replace P with (P ᴳ+ ᴳ{}). 2:{ crush. }
+    apply Ty_term_Map with (T := ①).
+    + apply Disjoint_empty_l.
+    + assumption.
+    + rewrite stimes_empty_eq, union_commutative. apply Ty_term_PatU.
+      * rewrite union_empty_l_eq with (G := ᴳ{ 0 : ¹ν ‗ ①}). apply Ty_term_Var. { apply DisposableOnly_empty. } { apply Disjoint_empty_l. } { repeat constructor. }
+      * rewrite union_empty_l_eq with (G := ᴳ{}). apply Ty_term_Val. { apply DisposableOnly_empty. } { rewrite <- stimes_empty_eq with (m := ¹∞). apply TyR_val_E. apply TyR_val_U. repeat constructor. } { apply DestOnly_empty. }
+  - replace (ᴳ{} ᴳ+ ᴳ{ 1 : ¹ν ‗ T} ᴳ+ ᴳ{ 2 : ¹ν ‗ ! ¹∞ ⁔ ①}) with (¹ν ᴳ· ᴳ{ 2 : ¹ν ‗ ! ¹∞ ⁔ ①} ᴳ+ ᴳ{ 1 : ¹ν ‗ T}). 2:{ crush. }
+    apply Ty_term_PatE with (T := ①).
+    + repeat constructor.
+    + repeat constructor.
+    + apply Disjoint_singletons_iff. sfirstorder.
+    + rewrite union_empty_l_eq with (G := ᴳ{ 2 : ¹ν ‗ ! ¹∞ ⁔ ①}). apply Ty_term_Var. { apply DisposableOnly_empty. } { apply Disjoint_empty_l. } { repeat constructor. }
+    + rewrite union_commutative. apply Ty_term_PatU.
+      * cbn. rewrite union_empty_l_eq at 1. apply Ty_term_Var. { apply DisposableOnly_empty. } { apply Disjoint_empty_l. } { repeat constructor. }
+      * rewrite union_empty_l_eq with (G := ᴳ{ 1 : ¹ν ‗ T}). apply Ty_term_Var. { apply DisposableOnly_empty. }  { apply Disjoint_empty_l. } { repeat constructor. }
+Qed.
